refining proof state

LoCalSafety.v
@@ -312,6 +312,388 @@ Proof.
   intros. inversion H; subst. eauto.
 Qed.
 
+Definition tenv_equiv (G1 G2 : type_env) : Prop :=
+  forall x, lookup_tenv G1 x = lookup_tenv G2 x.
+
+Definition subst_pat_val (x : term_var) (s : val) (p : pat) : pat :=
+  match p with
+  | pat_clause K binds body =>
+      if existsb
+           (fun b => if term_var_eq_dec x (fst b) then true else false)
+           binds
+      then pat_clause K binds body
+      else pat_clause K binds (subst_val x s body)
+  end.
+
+Fixpoint subst_pats_val (x : term_var) (s : val) (ps : list pat) : list pat :=
+  match ps with
+  | nil => nil
+  | p :: ps' => subst_pat_val x s p :: subst_pats_val x s ps'
+  end.
+
+Lemma lookup_tenv_app :
+  forall G1 G2 x,
+    lookup_tenv ((G1 ++ G2)%list) x =
+    match lookup_tenv G1 x with
+    | Some t => Some t
+    | None => lookup_tenv G2 x
+    end.
+Proof.
+  induction G1 as [| [y t] G1 IH]; intros G2 x; simpl.
+  - reflexivity.
+  - destruct (term_var_eq_dec x y); auto.
+Qed.
+
+Lemma in_lookup_tenv :
+  forall G x t,
+    In (x, t) G ->
+    exists t', lookup_tenv G x = Some t'.
+Proof.
+  induction G as [| [y u] G IH]; intros x t Hin; simpl in *.
+  - contradiction.
+  - destruct Hin as [Heq | Hin].
+    + inversion Heq; subst.
+      destruct (term_var_eq_dec x x); [eexists; reflexivity | contradiction].
+    + destruct (term_var_eq_dec x y).
+      * eexists; reflexivity.
+      * apply IH in Hin as [t' Hlk]. exists t'. exact Hlk.
+Qed.
+
+Lemma extend_tenv_list_rev :
+  forall G binds,
+    extend_tenv_list G binds = (rev binds ++ G)%list.
+Proof.
+  intros G binds. revert G.
+  induction binds as [| b binds IH]; intros G; simpl.
+  - reflexivity.
+  - rewrite IH. rewrite <- app_assoc. reflexivity.
+Qed.
+
+Lemma tenv_equiv_extend :
+  forall G1 G2 x t,
+    tenv_equiv G1 G2 ->
+    tenv_equiv (extend_tenv G1 x t) (extend_tenv G2 x t).
+Proof.
+  unfold tenv_equiv, extend_tenv.
+  intros G1 G2 x t Heq y. simpl.
+  destruct (term_var_eq_dec y x); auto.
+Qed.
+
+Lemma tenv_equiv_extend_list :
+  forall G1 G2 binds,
+    tenv_equiv G1 G2 ->
+    tenv_equiv (extend_tenv_list G1 binds) (extend_tenv_list G2 binds).
+Proof.
+  intros G1 G2 binds Heq. revert G1 G2 Heq.
+  induction binds as [| b binds IH]; intros G1 G2 Heq; simpl.
+  - exact Heq.
+  - destruct b as [x t]. apply IH. apply tenv_equiv_extend. exact Heq.
+Qed.
+
+Lemma tenv_equiv_extend_shadow :
+  forall G x t1 t2,
+    tenv_equiv (extend_tenv (extend_tenv G x t2) x t1)
+               (extend_tenv G x t1).
+Proof.
+  unfold tenv_equiv, extend_tenv.
+  intros G x t1 t2 y. simpl.
+  destruct (term_var_eq_dec y x); auto.
+Qed.
+
+Lemma tenv_equiv_shadow_under_prefix :
+  forall prefix G x t,
+    lookup_tenv prefix x <> None ->
+    tenv_equiv ((prefix ++ (x, t) :: G)%list) ((prefix ++ G)%list).
+Proof.
+  unfold tenv_equiv.
+  intros prefix G x t Hprefix y.
+  rewrite !lookup_tenv_app.
+  destruct (lookup_tenv prefix y) eqn:Hlookup; auto.
+  simpl.
+  destruct (term_var_eq_dec y x) as [Heq | Hneq].
+  - subst. exfalso. apply Hprefix. exact Hlookup.
+  - destruct (term_var_eq_dec y x); [contradiction | reflexivity].
+Qed.
+
+Lemma closed_value_typing_any_context :
+  forall FDs DI Sigma C A N vl T,
+    has_type FDs DI nil Sigma C A N A N (e_val vl) T ->
+    forall G Sigma' C' A' N',
+      (forall lr tc, In (lr, tc) Sigma -> In (lr, tc) Sigma') ->
+      has_type FDs DI G Sigma' C' A' N' A' N' (e_val vl) T.
+Proof.
+  intros FDs DI Sigma C A N vl T Hv.
+  inversion Hv; subst; intros G Sigma' C' A' N' Hsigma.
+  - match goal with [ Hlookup : lookup_tenv nil _ = Some _ |- _ ] =>
+      simpl in Hlookup; discriminate
+    end.
+  - econstructor. eauto.
+Qed.
+
+Scheme has_type_ind' := Induction for has_type Sort Prop
+with pat_has_type_ind' := Induction for pat_has_type Sort Prop
+with pats_have_type_ind' := Induction for pats_have_type Sort Prop.
+
+Combined Scheme typing_mutind
+  from has_type_ind', pat_has_type_ind', pats_have_type_ind'.
+
+Lemma has_type_tenv_equiv :
+  (forall FDs DI G Sigma C A N A' N' e T,
+      has_type FDs DI G Sigma C A N A' N' e T ->
+      forall G', tenv_equiv G G' ->
+      has_type FDs DI G' Sigma C A N A' N' e T)
+  /\
+  (forall FDs DI tc_s G Sigma C A N A' N' T p,
+      pat_has_type FDs DI tc_s G Sigma C A N A' N' T p ->
+      forall G', tenv_equiv G G' ->
+      pat_has_type FDs DI tc_s G' Sigma C A N A' N' T p)
+  /\
+  (forall FDs DI tc_s G Sigma C A N A' N' T ps,
+      pats_have_type FDs DI tc_s G Sigma C A N A' N' T ps ->
+      forall G', tenv_equiv G G' ->
+      pats_have_type FDs DI tc_s G' Sigma C A N A' N' T ps).
+Proof.
+  apply typing_mutind.
+  - intros FDs DI G S0 C A N x tc l r Hlookup Hstore G' Heq.
+    apply T_Var.
+    + rewrite <- (Heq x). exact Hlookup.
+    + exact Hstore.
+  - intros FDs DI G S0 C A N r0 i l r tc Hstore G' Heq.
+    apply T_ConcreteLoc. exact Hstore.
+  - intros FDs DI G S0 C A N A' N' A'' N'' x e1 e2 tc1 l1 r1 tc2 l2 r2
+      Hty1 IH1 Hty2 IH2 G' Heq.
+    eapply T_Let.
+    + apply IH1. exact Heq.
+    + apply IH2. apply tenv_equiv_extend. exact Heq.
+  - intros FDs DI G S0 C A N A' N' r e t Hty IH G' Heq.
+    eapply T_LRegion. apply IH. exact Heq.
+  - intros FDs DI G S0 C A N A'' N'' l r e tc' l' r' Hnone Hfresh Hneq
+      Hty IH G' Heq.
+    eapply T_LLStart; eauto.
+  - intros FDs DI G S0 C A N A'' N'' l lprev r e tc'' l'' r''
+      Halloc Hnur Hfresh Hneq Hty IH G' Heq.
+    eapply T_LLTag; eauto.
+  - intros FDs DI G S0 C A N A'' N'' l l1 r tc_prev e tc' l' r'
+      Halloc Hstore Hnotin Hfresh Hneq Hty IH G' Heq.
+    eapply T_LLAfter; eauto.
+  - intros FDs DI G S0 C A N dc l r vs tc fieldtcs Hdc Hnur Hlen G' Heq.
+    eapply T_DataCon; eauto.
+  - intros FDs DI G S0 C A N f lrs vs tc l r f_locs f_params f_retty
+      f_regions f_body Hfd Hnur Halloc Hlen1 Hlen2 G' Heq.
+    eapply T_App; eauto.
+  - intros FDs DI G S0 C A N A' N' scrut ps tc_s l_s r_s t
+      Hscrut IHscrut Hcover Hps IHps G' Heq.
+    eapply T_Case.
+    + apply IHscrut. exact Heq.
+    + exact Hcover.
+    + apply IHps. exact Heq.
+  - intros FDs DI tc_s G S0 C A N A' N' dc binds body tc fieldtcs tc_res l r
+      Hdc Htc Hfields Hstore Hbody IHbody G' Heq.
+    eapply T_Pat; eauto.
+    apply IHbody. apply tenv_equiv_extend_list. exact Heq.
+  - intros FDs DI tc_s G S0 C A N t G' Heq.
+    constructor.
+  - intros FDs DI tc_s G S0 C A N A1 N1 A2 N2 t p ps Hpat IHpat Hps IHps G' Heq.
+    eapply T_PatsCons.
+    + apply IHpat. exact Heq.
+    + apply IHps. exact Heq.
+Qed.
+
+Corollary expr_has_type_tenv_equiv :
+  forall FDs DI G Sigma C A N A' N' e T,
+    has_type FDs DI G Sigma C A N A' N' e T ->
+    forall G', tenv_equiv G G' ->
+    has_type FDs DI G' Sigma C A N A' N' e T.
+Proof.
+  intros. destruct has_type_tenv_equiv as [Hexpr _]. eauto.
+Qed.
+
+Corollary pat_has_type_tenv_equiv :
+  forall FDs DI tc_s G Sigma C A N A' N' T p,
+    pat_has_type FDs DI tc_s G Sigma C A N A' N' T p ->
+    forall G', tenv_equiv G G' ->
+    pat_has_type FDs DI tc_s G' Sigma C A N A' N' T p.
+Proof.
+  intros. destruct has_type_tenv_equiv as [_ [Hpat _]].
+  eauto.
+Qed.
+
+Corollary pats_have_type_tenv_equiv :
+  forall FDs DI tc_s G Sigma C A N A' N' T ps,
+    pats_have_type FDs DI tc_s G Sigma C A N A' N' T ps ->
+    forall G', tenv_equiv G G' ->
+    pats_have_type FDs DI tc_s G' Sigma C A N A' N' T ps.
+Proof.
+  intros. destruct has_type_tenv_equiv as [_ [_ Hps]].
+  eauto.
+Qed.
+
+Lemma existsb_bind_hit :
+  forall x (binds : list (term_var * ty)),
+    existsb
+      (fun b => if term_var_eq_dec x (fst b) then true else false)
+      binds = true ->
+    exists t : ty, In (x, t) binds.
+Proof.
+  intros x0 binds. induction binds as [| [y t] binds IH]; intros Hhit; simpl in *.
+  - discriminate.
+  - destruct (term_var_eq_dec x0 y).
+    + exists t. left. subst. reflexivity.
+    + apply IH in Hhit as [t' Hin]. exists t'. right. exact Hin.
+Qed.
+
+Lemma existsb_bind_miss :
+  forall x (binds : list (term_var * ty)) t,
+    existsb
+      (fun b => if term_var_eq_dec x (fst b) then true else false)
+      binds = false ->
+    ~ In (x, t) binds.
+Proof.
+  intros x0 binds. induction binds as [| [y u] binds IH]; intros t Hmiss Hin; simpl in *.
+  - exact Hin.
+  - destruct (term_var_eq_dec x0 y) as [Heq | Hneq].
+    + discriminate.
+    + destruct Hin as [Hin | Hin].
+      * inversion Hin; subst. contradiction.
+      * eapply IH; eauto.
+Qed.
+
+Lemma in_extend_store_list :
+  forall S0 entries ent,
+    In ent S0 ->
+    In ent (extend_store_list S0 entries).
+Proof.
+  intros S0 entries ent Hin. revert S0 ent Hin.
+  induction entries as [| entry entries IH]; intros S0 ent Hin; simpl.
+  - exact Hin.
+  - apply IH. simpl. right. exact Hin.
+Qed.
+
+Lemma tenv_equiv_shadow_under_binds :
+  forall Gamma binds x vty,
+    (exists t, In (x, t) binds) ->
+    tenv_equiv (extend_tenv_list ((x, vty) :: Gamma) binds)
+               (extend_tenv_list Gamma binds).
+Proof.
+  intros Gamma binds x vty [t Hin].
+  repeat rewrite extend_tenv_list_rev.
+  apply tenv_equiv_shadow_under_prefix.
+  destruct (in_lookup_tenv (rev binds) x t) as [t' Hlookup].
+  - apply (proj1 (in_rev binds (x, t))). exact Hin.
+  - rewrite Hlookup. discriminate.
+Qed.
+
+Lemma lookup_tenv_extend_tenv_list_miss :
+  forall G binds x,
+    lookup_tenv G x = None ->
+    existsb
+      (fun b => if term_var_eq_dec x (fst b) then true else false)
+      binds = false ->
+    lookup_tenv (extend_tenv_list G binds) x = None.
+Proof.
+  intros G binds. revert G.
+  induction binds as [| [y t] binds IH]; intros G x Hlookup Hmiss; simpl in *.
+  - exact Hlookup.
+  - destruct (term_var_eq_dec x y) as [Heq | Hneq].
+    + discriminate.
+    + apply IH.
+      * simpl. destruct (term_var_eq_dec x y); [contradiction | exact Hlookup].
+      * exact Hmiss.
+Qed.
+
+Lemma tenv_equiv_shadow_under_binds_prefix :
+  forall prefix Gamma binds x t,
+    existsb
+      (fun b => if term_var_eq_dec x (fst b) then true else false)
+      binds = true ->
+    tenv_equiv (extend_tenv_list ((prefix ++ (x, t) :: Gamma)%list) binds)
+               (extend_tenv_list ((prefix ++ Gamma)%list) binds).
+Proof.
+  intros prefix Gamma binds x t Hhit.
+  repeat rewrite extend_tenv_list_rev.
+  replace ((rev binds ++ prefix ++ (x, t) :: Gamma)%list)
+    with ((((rev binds ++ prefix)%list) ++ (x, t) :: Gamma)%list).
+  2:{ rewrite <- app_assoc. reflexivity. }
+  replace ((rev binds ++ prefix ++ Gamma)%list)
+    with ((((rev binds ++ prefix)%list) ++ Gamma)%list).
+  2:{ rewrite <- app_assoc. reflexivity. }
+  apply tenv_equiv_shadow_under_prefix.
+  apply existsb_bind_hit in Hhit as [t' Hin].
+  destruct (in_lookup_tenv (rev binds) x t') as [t'' Hlookup].
+  - apply (proj1 (in_rev binds (x, t'))). exact Hin.
+  - rewrite lookup_tenv_app. rewrite Hlookup. discriminate.
+Qed.
+
+Lemma in_subst_pats_val :
+  forall dc binds body ps z s,
+    In (pat_clause dc binds body) ps ->
+    exists body',
+      In (pat_clause dc binds body') (subst_pats_val z s ps).
+Proof.
+  intros dc binds body ps z s Hin.
+  induction ps as [| [dc' binds' body''] ps IH]; simpl in *.
+  - contradiction.
+  - destruct Hin as [Heq | Hin].
+    + inversion Heq; subst.
+      exists
+        (if existsb
+              (fun b => if term_var_eq_dec z (fst b) then true else false)
+              binds
+         then body
+         else subst_val z s body).
+      left.
+      destruct
+        (existsb
+           (fun b => if term_var_eq_dec z (fst b) then true else false)
+           binds); reflexivity.
+    + destruct (IH Hin) as [body' Hin'].
+      exists body'. right. exact Hin'.
+Qed.
+
+Lemma pats_cover_subst_pats_val :
+  forall DI tc ps z s,
+    pats_cover DI tc ps ->
+    pats_cover DI tc (subst_pats_val z s ps).
+Proof.
+  intros DI tc ps z s Hcover K fts Hin.
+  destruct (Hcover K fts Hin) as [binds [body Hinps]].
+  destruct (in_subst_pats_val K binds body ps z s Hinps) as [body' Hin'].
+  exists binds, body'. exact Hin'.
+Qed.
+
+Lemma subst_case_pats_eq :
+  forall z s ps,
+    (let fix go_pats (ps : list pat) : list pat :=
+       match ps with
+       | nil => nil
+       | pat_clause K binds body :: ps' =>
+           (if existsb
+                 (fun b => if term_var_eq_dec z (fst b) then true else false)
+                 binds
+            then pat_clause K binds body
+            else pat_clause K binds (subst_val z s body))
+           :: go_pats ps'
+       end
+     in go_pats ps) = subst_pats_val z s ps.
+Proof.
+  intros z s ps.
+  induction ps as [| [K binds body] ps IH]; simpl.
+  - reflexivity.
+  - f_equal. exact IH.
+Qed.
+
+Lemma subst_val_case :
+  forall z s scrut ps,
+    subst_val z s (e_case scrut ps) =
+    e_case (subst_in_val z s scrut) (subst_pats_val z s ps).
+Proof.
+  intros z s scrut ps.
+  simpl. f_equal.
+  induction ps as [| [K binds body] ps IH]; simpl.
+  - reflexivity.
+  - rewrite IH. reflexivity.
+Qed.
+
 (* ================================================================= *)
 (* Lemma: Substitution  (thesis Appendix A, Lemma Substitution)       *)
 (*                                                                    *)
@@ -321,13 +703,216 @@ Qed.
 (* substitution.                                                      *)
 (* ================================================================= *)
 
+Definition subst_expr_case
+    FDs DI G Sigma C A N A' N' e T
+    (HT : has_type FDs DI G Sigma C A N A' N' e T) : Prop :=
+  forall prefix z uty Gamma s,
+    G = ((prefix ++ (z, uty) :: Gamma)%list) ->
+    lookup_tenv prefix z = None ->
+    has_type FDs DI nil Sigma C A N A N (e_val s) uty ->
+    has_type FDs DI (prefix ++ Gamma)%list Sigma C A N A' N' (subst_val z s e) T.
+
+Definition subst_pat_case
+    FDs DI tc_s G Sigma C A N A' N' T p
+    (HT : pat_has_type FDs DI tc_s G Sigma C A N A' N' T p) : Prop :=
+  forall prefix z uty Gamma s,
+    G = ((prefix ++ (z, uty) :: Gamma)%list) ->
+    lookup_tenv prefix z = None ->
+    has_type FDs DI nil Sigma C A N A N (e_val s) uty ->
+    pat_has_type FDs DI tc_s (prefix ++ Gamma)%list Sigma C A N A' N' T (subst_pat_val z s p).
+
+Definition subst_pats_case
+    FDs DI tc_s G Sigma C A N A' N' T ps
+    (HT : pats_have_type FDs DI tc_s G Sigma C A N A' N' T ps) : Prop :=
+  forall prefix z uty Gamma s,
+    G = ((prefix ++ (z, uty) :: Gamma)%list) ->
+    lookup_tenv prefix z = None ->
+    has_type FDs DI nil Sigma C A N A N (e_val s) uty ->
+    pats_have_type FDs DI tc_s (prefix ++ Gamma)%list Sigma C A N A' N' T (subst_pats_val z s ps).
+
+Lemma substitution_val_mutual :
+  (forall FDs DI G Sigma C A N A' N' e T
+      (HT : has_type FDs DI G Sigma C A N A' N' e T),
+      subst_expr_case FDs DI G Sigma C A N A' N' e T HT)
+  /\
+  (forall FDs DI tc_s G Sigma C A N A' N' T p
+      (HT : pat_has_type FDs DI tc_s G Sigma C A N A' N' T p),
+      subst_pat_case FDs DI tc_s G Sigma C A N A' N' T p HT)
+  /\
+  (forall FDs DI tc_s G Sigma C A N A' N' T ps
+      (HT : pats_have_type FDs DI tc_s G Sigma C A N A' N' T ps),
+      subst_pats_case FDs DI tc_s G Sigma C A N A' N' T ps HT).
+Proof.
+  apply typing_mutind.
+  - intros FDs DI G Sigma C A N x tc l r Hlookup Hstore.
+    unfold subst_expr_case.
+    intros prefix z uty Gamma s HG Hnone Hclosed.
+    subst G. simpl in *.
+    rewrite lookup_tenv_app in Hlookup.
+    destruct (lookup_tenv prefix x) eqn:Hprefix.
+    + destruct (term_var_eq_dec z x) as [Heq | Hneq].
+      * subst x. rewrite Hnone in Hprefix. discriminate.
+      * inversion Hlookup; subst. simpl.
+        apply T_Var.
+        -- rewrite lookup_tenv_app. rewrite Hprefix. reflexivity.
+        -- exact Hstore.
+    + simpl in Hlookup.
+      destruct (term_var_eq_dec x z) as [Heq | Hneq].
+      * subst x. inversion Hlookup; subst.
+        simpl. destruct (term_var_eq_dec z z); [| contradiction].
+        eapply closed_value_typing_any_context.
+        -- exact Hclosed.
+        -- intros lr tc' Hin. exact Hin.
+      * simpl. destruct (term_var_eq_dec z x) as [Heqzx | Hneqzx].
+        { exfalso. apply Hneq. symmetry. exact Heqzx. }
+        apply T_Var.
+        -- rewrite lookup_tenv_app. rewrite Hprefix. simpl.
+           destruct (term_var_eq_dec x z); [contradiction | exact Hlookup].
+        -- exact Hstore.
+  - intros FDs DI G Sigma C A N r0 i l r tc Hstore.
+    unfold subst_expr_case.
+    intros prefix z uty Gamma s HG Hnone Hclosed.
+    subst G. simpl. apply T_ConcreteLoc. exact Hstore.
+  - intros FDs DI G Sigma C A N A' N' A'' N'' x e1 e2 tc1 l1 r1 tc2 l2 r2
+      Hty1 IH1 Hty2 IH2.
+    unfold subst_expr_case.
+    intros prefix z uty Gamma s HG Hnone Hclosed.
+    subst G. simpl.
+    eapply T_Let.
+    + eapply IH1; eauto.
+    + destruct (term_var_eq_dec z x) as [Heq | Hneq].
+      * subst x. simpl.
+        eapply expr_has_type_tenv_equiv.
+        -- exact Hty2.
+        -- change (tenv_equiv
+                     ((((z, LocTy tc1 l1 r1) :: prefix) ++ (z, uty) :: Gamma)%list)
+                     ((((z, LocTy tc1 l1 r1) :: prefix) ++ Gamma)%list)).
+           apply tenv_equiv_shadow_under_prefix.
+           simpl. destruct (term_var_eq_dec z z); [discriminate | contradiction].
+      * simpl.
+        eapply IH2
+          with (prefix := (x, LocTy tc1 l1 r1) :: prefix)
+               (z := z) (uty := uty) (Gamma := Gamma) (s := s).
+        -- reflexivity.
+        -- simpl. destruct (term_var_eq_dec z x); [contradiction | exact Hnone].
+        -- eapply closed_value_typing_any_context.
+           ++ exact Hclosed.
+           ++ intros lr tc' Hin. simpl. right. exact Hin.
+  - intros FDs DI G Sigma C A N A' N' r e t Hty IH.
+    unfold subst_expr_case.
+    intros prefix z uty Gamma s HG Hnone Hclosed.
+    subst G. simpl.
+    eapply T_LRegion.
+    eapply IH; eauto.
+    eapply closed_value_typing_any_context.
+    + exact Hclosed.
+    + intros lr tc' Hin. exact Hin.
+  - intros FDs DI G Sigma C A N A'' N'' l r e tc' l' r' Halloc Hfresh Hneq
+      Hty IH.
+    unfold subst_expr_case.
+    intros prefix z uty Gamma s HG Hnone Hclosed.
+    subst G. simpl.
+    eapply T_LLStart; eauto.
+    eapply IH; eauto.
+    eapply closed_value_typing_any_context.
+    + exact Hclosed.
+    + intros lr tc'' Hin. exact Hin.
+  - intros FDs DI G Sigma C A N A'' N'' l lprev r e tc'' l'' r''
+      Halloc Hnur Hfresh Hneq Hty IH.
+    unfold subst_expr_case.
+    intros prefix z uty Gamma s HG Hnone Hclosed.
+    subst G. simpl.
+    eapply T_LLTag; eauto.
+    eapply IH; eauto.
+    eapply closed_value_typing_any_context.
+    + exact Hclosed.
+    + intros lr tc' Hin. exact Hin.
+  - intros FDs DI G Sigma C A N A'' N'' l l1 r tc_prev e tc' l' r'
+      Halloc Hstore Hnotin Hfresh Hneq Hty IH.
+    unfold subst_expr_case.
+    intros prefix z uty Gamma s HG Hnone Hclosed.
+    subst G. simpl.
+    eapply T_LLAfter; eauto.
+    eapply IH; eauto.
+    eapply closed_value_typing_any_context.
+    + exact Hclosed.
+    + intros lr tc'' Hin. exact Hin.
+  - intros FDs DI G Sigma C A N dc l r vs tc fieldtcs Hdc Hnur Hlen.
+    unfold subst_expr_case.
+    intros prefix z uty Gamma s HG Hnone Hclosed.
+    subst G. simpl.
+    eapply T_DataCon; eauto.
+    rewrite map_length. exact Hlen.
+  - intros FDs DI G Sigma C A N f lrs vs tc l r f_locs f_params f_retty
+      f_regions f_body Hfd Hnur Halloc Hlen1 Hlen2.
+    unfold subst_expr_case.
+    intros prefix z uty Gamma s HG Hnone Hclosed.
+    subst G. simpl.
+    eapply T_App; eauto.
+    rewrite map_length. exact Hlen2.
+  - intros FDs DI G Sigma C A N A' N' scrut ps tc_s l_s r_s t
+      Hscrut IHscrut Hcover Hps IHps.
+    unfold subst_expr_case.
+    intros prefix z uty Gamma s HG Hnone Hclosed.
+    subst G. rewrite subst_val_case.
+    eapply T_Case.
+    + eapply IHscrut; eauto.
+    + eapply pats_cover_subst_pats_val. exact Hcover.
+    + eapply IHps; eauto.
+  - intros FDs DI tc_s G Sigma C A N A' N' dc binds body tc fieldtcs tc_res l r
+      Hdc Htc Hfields Hstore Hbody IHbody.
+    unfold subst_pat_case.
+    intros prefix z uty Gamma s HG Hnone Hclosed.
+    subst G. simpl.
+    destruct
+      (existsb
+         (fun b : term_var * ty =>
+            if term_var_eq_dec z (fst b) then true else false)
+         binds) eqn:Hbinds.
+    + eapply T_Pat; eauto.
+      eapply expr_has_type_tenv_equiv.
+      * exact Hbody.
+      * apply tenv_equiv_shadow_under_binds_prefix. exact Hbinds.
+    + eapply T_Pat; eauto.
+      replace (extend_tenv_list ((prefix ++ Gamma)%list) binds)
+        with ((extend_tenv_list prefix binds ++ Gamma)%list).
+      * eapply IHbody
+          with (prefix := extend_tenv_list prefix binds)
+               (z := z) (uty := uty) (Gamma := Gamma) (s := s).
+        -- repeat rewrite extend_tenv_list_rev.
+           rewrite <- app_assoc. reflexivity.
+        -- apply lookup_tenv_extend_tenv_list_miss; assumption.
+        -- eapply closed_value_typing_any_context.
+           ++ exact Hclosed.
+           ++ intros ent tc' Hin. apply in_extend_store_list. exact Hin.
+      * repeat rewrite extend_tenv_list_rev.
+        rewrite <- app_assoc. reflexivity.
+  - intros FDs DI tc_s G Sigma C A N t.
+    unfold subst_pats_case.
+    intros prefix z uty Gamma s HG Hnone Hclosed.
+    subst G. simpl. constructor.
+  - intros FDs DI tc_s G Sigma C A N A1 N1 A2 N2 t p ps Hpat IHpat Hps IHps.
+    unfold subst_pats_case.
+    intros prefix z uty Gamma s HG Hnone Hclosed.
+    subst G. simpl.
+    eapply T_PatsCons.
+    + eapply IHpat; eauto.
+    + eapply IHps; eauto.
+      eapply closed_value_typing_any_context.
+      * exact Hclosed.
+      * intros lr tc' Hin. exact Hin.
+Qed.
+
 Lemma substitution_val :
   forall FDs DI Gamma x vty Sigma C A N A' N' e T v0,
     has_type FDs DI (cons (x, vty) Gamma) Sigma C A N A' N' e T ->
-    has_type FDs DI Gamma Sigma C A N A N (e_val v0) vty ->
+    has_type FDs DI nil Sigma C A N A N (e_val v0) vty ->
     has_type FDs DI Gamma Sigma C A N A' N' (subst_val x v0 e) T.
 Proof.
-Admitted.
+  intros FDs DI Gamma x vty Sigma C A N A' N' e T v0 HT Hclosed.
+  destruct substitution_val_mutual as [Hex _].
+  eapply Hex with (prefix := nil) (z := x) (uty := vty) (Gamma := Gamma) (s := v0); eauto.
+Qed.
 
 (* ================================================================= *)
 (* Theorem: Progress  (thesis §2.2.3, Lemma Progress)                *)
@@ -363,7 +948,7 @@ Proof.
 
   (* ---- T_Var ----
      Γ = nil, so In (x, _) nil is False. *)
-  1: { exfalso. simpl in H. exact H. }
+  1: { exfalso. simpl in H. discriminate. }
 
   (* ---- T_ConcreteLoc ----
      e = e_val (v_cloc ...), already a value. *)
@@ -448,8 +1033,8 @@ Proof.
     (* 1. Invert scrutinee typing *)
     inversion Htype; subst.
     - (* T_Var: impossible in empty Γ *)
-      match goal with [ Hin : In _ nil |- _ ] =>
-        simpl in Hin; contradiction end.
+      match goal with [ Hlookup : lookup_tenv nil _ = Some _ |- _ ] =>
+        simpl in Hlookup; discriminate end.
     - (* T_ConcreteLoc: scrut = v_cloc r0 i l r *)
       simpl in Hvwf.
       (* 2-3. map-store consistency *)
